Cslib.lean
@@ -33,11 +33,12 @@ import Cslib.Foundations.Data.OmegaSequence.Init
 import Cslib.Foundations.Data.OmegaSequence.Temporal
 import Cslib.Foundations.Data.Relation
 import Cslib.Foundations.Lint.Basic
+import Cslib.Foundations.Semantics.FLTS.Basic
+import Cslib.Foundations.Semantics.FLTS.FLTSToLTS
+import Cslib.Foundations.Semantics.FLTS.LTSToFLTS
+import Cslib.Foundations.Semantics.FLTS.Prod
 import Cslib.Foundations.Semantics.LTS.Basic
 import Cslib.Foundations.Semantics.LTS.Bisimulation
-import Cslib.Foundations.Semantics.LTS.FLTS
-import Cslib.Foundations.Semantics.LTS.FLTSToLTS
-import Cslib.Foundations.Semantics.LTS.LTSToFLTS
 import Cslib.Foundations.Semantics.LTS.Simulation
 import Cslib.Foundations.Semantics.LTS.TraceEq
 import Cslib.Foundations.Semantics.ReductionSystem.Basic
