Cslib/Computability/Automata/NA/ToDA.lean
@@ -6,7 +6,7 @@ Authors: Fabrizio Montesi
 
 import Cslib.Computability.Automata.DA.Basic
 import Cslib.Computability.Automata.NA.Basic
-import Cslib.Foundations.Semantics.LTS.LTSToFLTS
+import Cslib.Foundations.Semantics.FLTS.LTSToFLTS
 
 /-! # Translation of Nondeterministic Automata for finite strings into Deterministic Automata
 
