Cslib/Foundations/Semantics/FLTS/Prod.lean
@@ -1,0 +1,29 @@
+/-
+Copyright (c) 2025 Fabrizio Montesi. All rights reserved.
+Released under Apache 2.0 license as described in the file LICENSE.
+Authors: Ching-Tsun Chou, Fabrizio Montesi
+-/
+
+import Cslib.Foundations.Semantics.FLTS.Basic
+
+/-! # Product of functional labelled transition systems -/
+
+namespace Cslib.FLTS
+
+variable {State Label : Type*}
+
+/-- The product of two FLTS with the same label type. -/
+@[scoped grind =]
+def prod (flts1 : FLTS State1 Label) (flts2 : FLTS State2 Label) :
+    FLTS (State1 × State2) Label where
+  tr := fun (s1, s2) μ ↦ (flts1.tr s1 μ, flts2.tr s2 μ)
+
+/-- A state is reachable by the product FLTS iff its components are reachable by
+the respective FLTS components. -/
+@[simp, scoped grind =]
+theorem prod_mtr_eq (flts1 : FLTS State1 Label) (flts2 : FLTS State2 Label)
+    (s : State1 × State2) (μs : List Label) :
+    (flts1.prod flts2).mtr s μs = (flts1.mtr s.fst μs, flts2.mtr s.snd μs) := by
+  induction μs generalizing s <;> grind
+
+end Cslib.FLTS
